:PROPERTIES:
:ID:       e6f5dd9b-091e-4cfe-b351-4241b050b9a8
:END:
#+title: OU:M208:Unit-A3:Direct Proof:Proof By Induction
#+filetags: OU M208 Mathematics Proofs Statements Direct-Proof Induction

#+LATEX_HEADER: \usepackage{tcolorbox}

\begin{tcolorbox}[title=Principle of Mathematical Induction]
To prove that a statement $P(n)$ is true for $n = 1, 2, \ldots$:

\begin{itemize}
\item show that $P(1)$ is true
\item show that the implication $P(k) \implies P(k + 1)$ is true for $k = 1, 2, \ldots$
\end{itemize}
\end{tcolorbox}

For example:

 Prove that \(1 + 3 + \ldots + (2n - 1) = n^{2}\) for \(n = 1, 2, \ldots\).

 Let \(P(n)\) be the statement \(1 + 3 + \ldots + (2n - 1) = n^{2}\).

 \(P(1)\) is true because \(1 = 1^{2}\).

 Now let \(k \ge 1\) and assume \(P(k)\) is true, that is:

 \(1 + 3 + \ldots + (2k - 1) = k^{2}\)

 We want to deduce that \(P(k+1)\) is true, that is:

 \(1 + 3 + \ldots + (2k - 1) + (2k + 1) = (k+1)^{2}\)

 Then:

 \begin{align*}
1 + 3 + \ldots + (2k - 1) + (2k + 1) &= (1 + 3 + \ldots + (2k - 1)) + (2k + 1) \\
                                &= k^{2} + (2k + 1) \\
                                &= (k + 1)^{2} \\
 \end{align*}
