:PROPERTIES:
:ID:       e632b886-54fd-446e-9f73-8122f136206d
:END:
#+title: OU:M208:Unit-A2:Complex Numbers:Complex Conjugate
#+filetags: OU M208 Mathematics Complex-Numbers Complex-Conjugate

#+LATEX_HEADER: \usepackage{tcolorbox}

\begin{tcolorbox}[title=The Complex Conjugate]
The \textbf{complex conjugate} $\overline{z}$ of the complex number $z = x + iy$ is the complex number $x - iy$.
\end{tcolorbox}

  * For example, the complex conjugate of $z = 1 - 2i$ is \(\overline{z} = 1 + 2i\)

The folowing useful properties apply to complex conjugations:

\begin{tcolorbox}[title=Properties of Complex Conjugates]
Let $z_1, z_2$ and $z$ be any complex numbers. Then:

\begin{enumerate}
\item $\overline{z_1 + z_2} = \overline{z_1} + \overline{z_2}$
\item $\overline{z_1z_2} = \overline{z_1} \times \overline{z_2}$
\item $z + \overline{z} = 2\text{Re}\ z$
\item $z - \overline{z} = 2\text{Im}\ z$
\end{enumerate}
\end{tcolorbox}

- For the following proofs, see [[id:6274d52c-220c-4342-afe2-01b869ea0609][OU:M208:Unit-A2:Complex Numbers:Arithmetic of Complex Numbers]] to understand why the operations are expanded in this way.

* Proof of property 1

\begin{align*}
\overline{z_1 + z_2} &= \overline{(x_1 + x_2) + i(y_1 + y_2)} \\
                     &= (x_1 + x_2) - i(y_1 + y_2) \\
                     &= (x_1 + x_2) - iy_1 - iy_2 \\
                     &= (x_1 - iy_1) + (x_2 - iy_2) \\
                     &= \overline{z_1} + \overline{z_2}
\end{align*}

* Proof of property 2

\begin{align*}
\overline{z_1z_2} &= \overline{(x_1x_2 - y_1y_2) + i(x_2y_1 - x_1y_2)} \\
                  &= (x_1x_2 - y_1y_2) - i(x_2y_1 - x_1y_2) \\
                  &= x_1x_2 - y_1y_2 - ix_2y_1 + ix_1y_2 \\
                  &= x_1x_2 + i^2y_1y_2 - ix_2y_1 + ix_1y_2 \\
                  &= (x_1 - iy_1)(x_2 - iy_2) \\
                  &= \overline{z_1}\times\overline{z_2}
\end{align*}

* Proof of property 3

\begin{align*}
z + \overline{z} &= (x + iy) + \overline{(x + iy)} \\
                 &= (x + iy) + (x - iy) \\
                 &= x + iy + x - iy \\
                 &= 2x \\
                 &= 2\text{Re}\ z
\end{align*}

* Proof of property 4

\begin{align*}
z - \overline{z} &= (x + iy) - \overline{(x + iy)} \\
                 &= (x + iy) - (x - iy) \\
                 &= x + iy - x + iy \\
                 &= 2iy \\
                 &= 2i\text{Im}\ z
\end{align*}
